![[Pasted image 20250113103159.png]]

## a
$$
a \implies b
$$
$$
\lnot a \lor b \iff b \lor \lnot a
$$
$$
\lnot b \implies \lnot a
$$
$$
\forall a,b \in K: a\not=0\land b\not=0 \implies a\cdot b\not=0
$$
$$

$$

## b
$\forall a,d\in K~~(a,0)\cdot(0,d)=(0,0)$
nicht erf√ºllt

## 2
$$
\left(\begin{matrix}
1 \\
2 \\
-3 \\
0
\end{matrix}\right)
,\left(\begin{matrix}
1 \\
1 \\
3 \\
0
\end{matrix}\right)
,\left(\begin{matrix}
1 \\
2 \\
-3 \\
1
\end{matrix}\right)
$$

$$
\left(\begin{matrix}
1 | 1 | 1 \\
2 |2 |1 \\
-3 | -3 | 3 \\
1 | 0 | 0
\end{matrix}\right)
\rightarrow z_{3}=z_{3}-3z_{1}\left(\begin{matrix}
1|1|1 \\
2|2|1 \\
-6 | -6 | 0 \\
1 | 0 | 0
\end{matrix}\right)
$$
$$
\left(\begin{matrix}
1 | 1| 1 \\
1 | 2 | 2 \\
0 | -6 |-6 \\
0 |0 |1
\end{matrix}\right)
$$
## 3 a
## 3b